first version of Lean

LeanCourse/Basic.lean
@@ -1,1 +1,28 @@
-def hello := "world"
+set_option autoImplicit true
+
+inductive Struct (α β γ : Type u) where
+  | mtst : Struct α β γ
+  | var (val : α) : Struct α β γ
+  | store (st : Struct α β γ) (k : β ⊕ γ) (v : Struct α β γ) : Struct α β γ
+
+open Struct
+
+def save (st : Struct α β γ) (fields : List Nat) (v : Struct α β γ) : Struct α β γ :=
+  match st, fields with
+  | mtst, [] => sorry
+  | mtst, k :: rest => store mtst k $ inl $ save mtst rest v
+  | store st k v, [] => store st k v
+  | store st k (inr v'), xs@(k' :: _) =>
+    if k = k' then store st k (inr v') else store (save st xs v) k (inr v')
+  | store st k (inl v'), xs@(k' :: rest) =>
+    if k = k' then store st k (inl $ save v' rest v) else store (save st xs v) k (inl v')
+
+def select (st : Struct α β γ) (k : Nat) : Struct α β γ :=
+  match st with
+  | mtst => mtst
+  | store st k' v => if k = k' then v else select st k'
+
+theorem selectSave (st : Struct α β γ) (k : Nat) (path : List Nat) (v : Struct α β γ) (k' : Nat) :
+  select (save st (k :: path) v) k' =
+  (if k = k' then save (select st k') path v else select st k') := by
+  sorry
